Filled in Substitution, Reduction, and Typing rules for MoreStlc.  Added examples and stubbed their proofs.  Added stubs proofs for properties.

SoftwareFoundations/ProgrammingLanguageFoundations/MoreStlc.lean
@@ -2,6 +2,9 @@
 # More on the Simply-Typed Lambda Calculus
 -/
 
+import SoftwareFoundations.LogicalFoundations.Maps
+import SoftwareFoundations.ProgrammingLanguageFoundations.SmallStep
+
 namespace SoftwareFoundations.ProgrammingLanguageFoundations.MoreStlc
   /-
   ## Simple Extensions to the STLC
@@ -22,6 +25,10 @@ namespace SoftwareFoundations.ProgrammingLanguageFoundations.MoreStlc
   ## Exercise: Formalizing the Extensions
   -/
 
+  /-
+  #### Syntaxs
+  -/
+
   inductive Ty: Type where
     | unit: Ty
     | bool: Ty
@@ -39,6 +46,7 @@ namespace SoftwareFoundations.ProgrammingLanguageFoundations.MoreStlc
     syntax:max "ℕ" : stlc_ty
     syntax:max "‹" term "›" : stlc_ty
 
+    syntax:50 "()" : stlc_ty
     syntax:50 stlc_ty:50 "×" stlc_ty:51 : stlc_ty
     syntax:50 stlc_ty:50 "+" stlc_ty:51 : stlc_ty
     syntax:50 "[" stlc_ty "]" : stlc_ty
@@ -52,6 +60,7 @@ namespace SoftwareFoundations.ProgrammingLanguageFoundations.MoreStlc
     macro_rules
       | `([Ty| 𝔹])          => `(Ty.bool)
       | `([Ty| ℕ])          => `(Ty.nat)
+      | `([Ty| ()])         => `(Ty.unit)
       | `([Ty| ‹$ty:term›]) => `($(Lean.quote ty))
       | `([Ty| $t₁ × $t₂])  => `(Ty.prod [Ty| $t₁] [Ty| $t₂])
       | `([Ty| $t₁ + $t₂])  => `(Ty.sum [Ty| $t₁] [Ty| $t₂])
@@ -63,6 +72,7 @@ namespace SoftwareFoundations.ProgrammingLanguageFoundations.MoreStlc
   section
     example: [Ty| 𝔹] = Ty.bool := rfl
     example: [Ty| ℕ] = Ty.nat := rfl
+    example: [Ty| ()] = Ty.unit := rfl
     example {t:Ty}: [Ty| ‹t›] = t := rfl
 
     example: [Ty| ℕ × ℕ] = Ty.prod .nat .nat := rfl
@@ -113,7 +123,7 @@ namespace SoftwareFoundations.ProgrammingLanguageFoundations.MoreStlc
 
     | ite (c t f: Term): Term
 
-    | inl (ty: Ty) (t: Term): Term
+    | inl (t: Term) (ty: Ty): Term
     | inr (ty: Ty) (t: Term): Term
     | scase (s: Term) (p₁: String) (b₁: Term) (id₂: String) (b₂: Term): Term
 
@@ -178,8 +188,8 @@ namespace SoftwareFoundations.ProgrammingLanguageFoundations.MoreStlc
 
     syntax "ite" stlc "then" stlc "else" stlc : stlc
 
-    syntax "inl" stlc ":" stlc_ty : stlc
-    syntax "inr" stlc ":" stlc_ty : stlc
+    syntax "inl" "(" stlc "|" stlc_ty ")" : stlc
+    syntax "inr" "(" stlc_ty "|" stlc ")" : stlc
     syntax "case" stlc "of" "|" "inl" ident "⇒" stlc "|" "inr" ident "⇒" stlc : stlc
     syntax "case" stlc "of" "|" "inl" ident "⇒" stlc "|" "inr" "‹" term "›" "⇒" stlc : stlc
     syntax "case" stlc "of" "|" "inl" "‹" term "›" "⇒" stlc "|" "inr" ident "⇒" stlc : stlc
@@ -248,8 +258,8 @@ namespace SoftwareFoundations.ProgrammingLanguageFoundations.MoreStlc
 
       | `([Term| ite $c then $t else $f])                                         => `(Term.ite [Term| $c] [Term| $t] [Term| $f])
 
-      | `([Term| inl $t : $ty])                                                   => `(Term.inl [Ty| $ty] [Term| $t])
-      | `([Term| inr $t : $ty])                                                   => `(Term.inr [Ty| $ty] [Term| $t])
+      | `([Term| inl ( $t | $ty )])                                               => `(Term.inl [Term| $t] [Ty| $ty])
+      | `([Term| inr ( $ty | $t )])                                               => `(Term.inr [Ty| $ty] [Term| $t])
       | `([Term| case $s of | inl $id₁ ⇒ $t₁ | inr $id₂ ⇒ $t₂])                   => `(Term.scase [Term| $s] $(Lean.quote (toString (id₁).getId)) [Term| $t₁] $(Lean.quote (toString (id₂).getId)) [Term| $t₂])
       | `([Term| case $s of | inl $id₁ ⇒ $t₁ | inr ‹ $id₂:term › ⇒ $t₂])          => `(Term.scase [Term| $s] $(Lean.quote (toString (id₁).getId)) [Term| $t₁] $(Lean.quote id₂) [Term| $t₂])
       | `([Term| case $s of | inl ‹ $id₁:term › ⇒ $t₁ | inr $id₂ ⇒ $t₂])          => `(Term.scase [Term| $s] $(Lean.quote id₁) [Term| $t₁] $(Lean.quote (toString (id₂).getId)) [Term| $t₂])
@@ -411,10 +421,10 @@ namespace SoftwareFoundations.ProgrammingLanguageFoundations.MoreStlc
     example: [Term| ite ‹c› ‹t₁› ‹t₂› then ‹t› ‹t₃› ‹t₄› else ‹f› ‹t₅› ‹t₆›] = Term.ite (.app (.app c t₁) t₂) (.app (.app t t₃) t₄) (.app (.app f t₅) t₆) := rfl
     example: [Term| ite ‹t₁› ∧ ‹t₂› then ‹t₃› ∨ ‹t₄› else ‹t₅› ≠ ‹t₆›] = Term.ite (.and t₁ t₂) (.or t₃ t₄) (.neq t₅ t₆) := rfl
 
-    example: [Term| inl 42: ℕ] = Term.inl .nat (.const 42) := rfl
-    example: [Term| inr tru: 𝔹] = Term.inr .bool .true := rfl
-    example: [Term| inl 1 + 2: ℕ ∧ inr ¬ tru: 𝔹] = Term.and (.inl .nat (.add (.const 1) (.const 2))) (.inr .bool (.not .true)) := rfl
-    example: [Term| inl 1 + 2: ℕ ≠ inr ¬ tru: 𝔹] = Term.neq (.inl .nat (.add (.const 1) (.const 2))) (.inr .bool (.not .true)) := rfl
+    example: [Term| inl (42 | ℕ)] = Term.inl (.const 42) .nat := rfl
+    example: [Term| inr (𝔹 | tru)] = Term.inr .bool .true := rfl
+    example: [Term| inl (1 + 2 | ℕ) ∧ inr (𝔹 | ¬ tru)] = Term.and (.inl (.add (.const 1) (.const 2)) .nat) (.inr .bool (.not .true)) := rfl
+    example: [Term| inl (1 + 2 | ℕ) ≠ inr (𝔹 | ¬ tru)] = Term.neq (.inl (.add (.const 1) (.const 2)) .nat) (.inr .bool (.not .true)) := rfl
     example: [Term| case ‹t₁› of | inl x ⇒ ‹t₂› | inr y ⇒ ‹t₃›] = Term.scase t₁ "x" t₂ "y" t₃ := rfl
     example: [Term| case ‹t₁› of | inl ‹id₁› ⇒ ‹t₂› | inr y ⇒ ‹t₃›] = Term.scase t₁ id₁ t₂ "y" t₃ := rfl
     example: [Term| case ‹t₁› of | inl x ⇒ ‹t₂› | inr ‹id₂› ⇒ ‹t₃›] = Term.scase t₁ "x" t₂ id₂ t₃ := rfl
@@ -457,4 +467,570 @@ namespace SoftwareFoundations.ProgrammingLanguageFoundations.MoreStlc
     example: [Term| fix ‹t₁›] = Term.fix t₁ := rfl
     example: [Term| fix (λ ‹id₁›: ℕ. ‹t₁›)] = Term.fix (.abs id₁ .nat t₁) := rfl
   end
+
+  /-
+  #### Substitution
+  -/
+
+  @[reducible]
+  def Term.subst (id: String) (s: Term): Term → Term
+    | .var v     => if id = v then s else .var v
+    | .abs v t b => if id = v then .abs v t b else .abs v t (subst id s b)
+    | .app f x   => .app (subst id s f) (subst id s x)
+
+    | .true        => .true
+    | .false       => .false
+    | .and t₁ t₂   => .and (subst id s t₁) (subst id s t₂)
+    | .or t₁ t₂    => .or (subst id s t₁) (subst id s t₂)
+    | .not t       => .not (subst id s t)
+    | .bcase c t f => .bcase (subst id s c) (subst id s t) (subst id s f)
+
+    | .const n   => .const n
+    | .pred t    => .pred (subst id s t)
+    | .succ t    => .succ (subst id s t)
+    | .add t₁ t₂ => .add (subst id s t₁) (subst id s t₂)
+    | .sub t₁ t₂ => .sub (subst id s t₁) (subst id s t₂)
+    | .mul t₁ t₂ => .mul (subst id s t₁) (subst id s t₂)
+    | .div t₁ t₂ => .div (subst id s t₁) (subst id s t₂)
+    | .mod t₁ t₂ => .mod (subst id s t₁) (subst id s t₂)
+    | .exp t₁ t₂ => .exp (subst id s t₁) (subst id s t₂)
+
+    | .eq t₁ t₂  => .eq (subst id s t₁) (subst id s t₂)
+    | .neq t₁ t₂ => .neq (subst id s t₁) (subst id s t₂)
+    | .lt t₁ t₂  => .lt (subst id s t₁) (subst id s t₂)
+    | .le t₁ t₂  => .le (subst id s t₁) (subst id s t₂)
+    | .gt t₁ t₂  => .gt (subst id s t₁) (subst id s t₂)
+    | .ge t₁ t₂  => .ge (subst id s t₁) (subst id s t₂)
+
+    | .ite c t f => .ite (subst id s c) (subst id s t) (subst id s f)
+
+    | .inl t ty              => .inl (subst id s t) ty
+    | .inr ty t              => .inr ty (subst id s t)
+    | .scase c id₁ b₁ id₂ b₂ =>
+      let b₁ := if id₁ = id then b₁ else subst id s b₁
+      let b₂ := if id₂ = id then b₂ else subst id s b₂
+      .scase (subst id s c) id₁ b₁ id₂ b₂
+
+    | .nil                 => .nil
+    | .cons hd tl          => .cons (subst id s hd) (subst id s tl)
+    | .lcase l b₁ hd tl b₂ =>
+      let b₂ := if id = hd ∨ id = tl then b₂ else subst id s b₂
+      .lcase (subst id s l) (subst id s b₁) hd tl b₂
+
+    | .unit => .unit
+
+    | .pair l r          => .pair (subst id s l) (subst id s r)
+    | .fst p             => .fst (subst id s p)
+    | .snd p             => .snd (subst id s p)
+    | .pcase p id₁ id₂ b =>
+      let b := if id = id₁ ∨ id = id₂ then b else subst id s b
+      .pcase p id₁ id₂ b
+
+    | .let v t₁ t₂ =>
+      if id = v
+      then .let v t₁ t₂
+      else .let v (subst id s t₁) (subst id s t₂)
+
+    | .fix f => .fix (subst id s f)
+
+  scoped notation "[" id "↦" s "]" t => Term.subst id s t
+
+  section
+    example: (["z" ↦ (.const 0)] [Term| (λ x: 𝔹. z)]) = [Term| λ x: 𝔹. 0] := rfl
+    example: (["z" ↦ (.const 0)] [Term| (λ z: 𝔹. z)]) = [Term| λ z: 𝔹. z] := rfl
+
+    example: (["z" ↦ (.const 0)] [Term| case tru of | tru ⇒ z | fls ⇒ z]) = [Term| case tru of | tru ⇒ 0 | fls ⇒ 0] := rfl
+
+    example: (["z" ↦ (.const 0)] [Term| case x of | inl l ⇒ z | inr r ⇒ z]) = [Term| case x of | inl l ⇒ 0 | inr r ⇒ 0] := rfl
+    example: (["z" ↦ (.const 0)] [Term| case x of | inl l ⇒ z | inr z ⇒ z]) = [Term| case x of | inl l ⇒ 0 | inr z ⇒ z] := rfl
+    example: (["z" ↦ (.const 0)] [Term| case x of | inl z ⇒ z | inr r ⇒ z]) = [Term| case x of | inl z ⇒ z | inr r ⇒ 0] := rfl
+    example: (["z" ↦ (.const 0)] [Term| case x of | inl z ⇒ z | inr z ⇒ z]) = [Term| case x of | inl z ⇒ z | inr z ⇒ z] := rfl
+
+    example: (["z" ↦ (.const 0)] [Term| case [] of | nil ⇒ z | hd::tl ⇒ z]) = [Term| case [] of | nil ⇒ 0 | hd::tl ⇒ 0] := rfl
+    example: (["z" ↦ (.const 0)] [Term| case [] of | nil ⇒ z | hd::z ⇒ z]) = [Term| case [] of | nil ⇒ 0 | hd::z ⇒ z] := rfl
+    example: (["z" ↦ (.const 0)] [Term| case [] of | nil ⇒ z | z::tl ⇒ z]) = [Term| case [] of | nil ⇒ 0 | z::tl ⇒ z] := rfl
+    example: (["z" ↦ (.const 0)] [Term| case [] of | nil ⇒ z | z::z ⇒ z]) = [Term| case [] of | nil ⇒ 0 | z::z ⇒ z] := rfl
+
+    example: (["z" ↦ (.const 0)] [Term| case (x, y) of | (l, r) ⇒ z]) = [Term| case (x, y) of | (l, r) ⇒ 0] := rfl
+    example: (["z" ↦ (.const 0)] [Term| case (x, y) of | (l, z) ⇒ z]) = [Term| case (x, y) of | (l, z) ⇒ z] := rfl
+    example: (["z" ↦ (.const 0)] [Term| case (x, y) of | (z, r) ⇒ z]) = [Term| case (x, y) of | (z, r) ⇒ z] := rfl
+    example: (["z" ↦ (.const 0)] [Term| case (x, y) of | (z, z) ⇒ z]) = [Term| case (x, y) of | (z, z) ⇒ z] := rfl
+
+    example: (["z" ↦ (.const 0)] [Term| let w = z in z]) = [Term| let w = 0 in 0] := rfl
+    example: (["z" ↦ (.const 0)] [Term| let w = z in w]) = [Term| let w = 0 in w] := rfl
+    example: (["z" ↦ (.const 0)] [Term| let y = succ 0 in z]) = [Term| let y = succ 0 in 0] := rfl
+  end
+
+  inductive Subst (id: String) (s: Term): Term → Term → Prop where
+
+  namespace Term
+    theorem Subst.correct {id: String} {s t₁ t₂: Term}: ([id ↦ s] t₁) = t₂ ↔ Subst id s t₁ t₂ := sorry
+  end Term
+
+  namespace Tactic
+    theorem Subst.correct {id: String} {s t₁ t₂: Term}: ([id ↦ s] t₁) = t₂ ↔ Subst id s t₁ t₂ := by sorry
+  end Tactic
+
+  namespace Blended
+    theorem Subst.correct {id: String} {s t₁ t₂: Term}: ([id ↦ s] t₁) = t₂ ↔ Subst id s t₁ t₂ := sorry
+  end Blended
+
+  /-
+  #### Reduction
+  -/
+
+  inductive Value: Term → Prop where
+    | true: Value [Term| tru]
+    | false: Value [Term| fls]
+    | const {n: Nat}: Value [Term| ‹nat:n›]
+    | abs {id: String} {ty: Ty} {b: Term}: Value [Term| λ ‹id›: ‹ty›. ‹b›]
+    | inl {ty: Ty} {t: Term} (h₁: Value t): Value [Term| inl (‹t› | ‹ty›)]
+    | inr {ty: Ty} {t: Term} (h₁: Value t): Value [Term| inr (‹ty› | ‹t›)]
+    | nil: Value [Term| []]
+    | cons {t₁ t₂: Term} (h₁: Value t₁) (h₂: Value t₂): Value [Term| ‹t₁› :: ‹t₂›]
+    | unit: Value [Term| ()]
+    | pair {t₁ t₂: Term} (h₁: Value t₁) (h₂: Value t₂): Value [Term| (‹t₁›, ‹t₂›)]
+
+  inductive Eq: Term → Term → Prop where
+    | true: Eq [Term| tru] [Term| tru]
+    | false: Eq [Term| fls] [Term| fls]
+    | const {n₁ n₂: Nat} (h₁: n₁ = n₂): Eq [Term| ‹nat:n₁›] [Term| ‹nat:n₂›]
+    | inl {t₁ t₂: Term} {ty₁ ty₂: Ty} (h₁: Value t₁) (h₂: Value t₂) (h₃: Eq t₁ t₂) (h₄: ty₁ = ty₂): Eq [Term| inl (‹t₁› | ‹ty₁›)] [Term| inl (‹t₂› | ‹ty₂›)]
+    | inr {t₁ t₂: Term} {ty₁ ty₂: Ty} (h₁: Value t₁) (h₂: Value t₂) (h₃: Eq t₁ t₂) (h₄: ty₁ = ty₂): Eq [Term| inr (‹ty₁› | ‹t₁›)] [Term| inr (‹ty₂› | ‹t₂›)]
+    | nil: Eq [Term| []] [Term| []]
+    | cons {hd₁ hd₂ tl₁ tl₂: Term} (h₁: Value hd₁) (h₂: Value hd₂) (h₃: Value tl₁) (h₄: Value tl₂) (h₅: Eq hd₁ hd₂) (h₆: Eq tl₁ tl₂): Eq [Term| ‹hd₁› :: ‹tl₁›] [Term| ‹hd₂› :: ‹tl₂›]
+    | unit: Eq [Term| ()] [Term| ()]
+    | pair {f₁ f₂ s₁ s₂: Term} (h₁: Value f₁) (h₂: Value f₂) (h₃: Value s₁) (h₄: Value s₂) (h₅: Eq f₁ f₂) (h₆: Eq s₁ s₂): Eq [Term| (‹f₁›, ‹s₁›)] [Term| (‹f₂›, ‹s₂›)]
+
+  inductive Eval₁: Term → Term → Prop where
+    | appL {t₁ t₂ t₃: Term} (h₁: Eval₁ t₁ t₂): Eval₁ [Term| ‹t₁› ‹t₃›] [Term| ‹t₂› ‹t₃›]
+    | appR {v₁ t₁ t₂: Term} (h₁: Value v₁) (h₂: Eval₁ t₁ t₂): Eval₁ [Term| ‹v₁› ‹t₁›] [Term| ‹v₁› ‹t₂›]
+    | appAbs {id: String} {t: Ty} {b x: Term} (h₁: Value x): Eval₁ [Term| (λ ‹id›: ‹ty›. ‹b›) ‹x›] ([id ↦ x] [Term| ‹b›])
+
+    | andL {t₁ t₂ t₃: Term} (h₁: Eval₁ t₁ t₂): Eval₁ [Term| ‹t₁› ∧ ‹t₃›] [Term| ‹t₂› ∧ ‹t₃›]
+    | andR {v₁ t₁ t₂: Term} (h₁: Value v₁) (h₂: Eval₁ t₁ t₂): Eval₁ [Term| ‹v₁› ∧ ‹t₁›] [Term| ‹v₂› ∧ ‹t₂›]
+    | andTrueTrue: Eval₁ [Term| tru ∧ tru] [Term| tru]
+    | andTrueFalse: Eval₁ [Term| tru ∧ fls] [Term| fls]
+    | andFalseTrue: Eval₁ [Term| fls ∧ tru] [Term| fls]
+    | andFalseFalse: Eval₁ [Term| fls ∧ fls] [Term| fls]
+    | orL {t₁ t₂ t₃: Term} (h₁: Eval₁ t₁ t₂): Eval₁ [Term| ‹t₁› ∨ ‹t₃›] [Term| ‹t₂› ∨ ‹t₃›]
+    | orR {v₁ t₁ t₂: Term} (h₁: Value v₁) (h₂: Eval₁ t₁ t₂): Eval₁ [Term| ‹v₁› ∨ ‹t₁›] [Term| ‹v₂› ∨ ‹t₂›]
+    | orTrueTrue: Eval₁ [Term| tru ∧ tru] [Term| tru]
+    | orTrueFalse: Eval₁ [Term| tru ∧ fls] [Term| tru]
+    | orFalseTrue: Eval₁ [Term| fls ∧ tru] [Term| tru]
+    | orFalseFalse: Eval₁ [Term| fls ∧ fls] [Term| fls]
+    | notStep {t₁ t₂: Term} (h₁: Eval₁ t₁ t₂): Eval₁ [Term| ¬ ‹t₁›] [Term| ¬ ‹t₂›]
+    | notTrue: Eval₁ [Term| ¬ tru] [Term| fls]
+    | notFalse: Eval₁ [Term| ¬ fls] [Term| tru]
+    | bcaseTrue {t f: Term}: Eval₁ [Term| case tru of | tru ⇒ ‹t› | fls ⇒ ‹f›] [Term| ‹t›]
+    | bcaseFalse {t f: Term}: Eval₁ [Term| case fls of | tru ⇒ ‹t› | fls ⇒ ‹f›] [Term| ‹f›]
+    | bcase {c₁ c₂ t f: Term} (h₁: Eval₁ c₁ c₂): Eval₁ [Term| case ‹c₁› of | tru ⇒ ‹t› | fls ⇒ ‹f›] [Term| case ‹c₂› of | tru ⇒ ‹t› | fls ⇒ ‹f›]
+
+    | succConst {n: Nat}: Eval₁ [Term| succ ‹nat:n›] [Term| ‹nat:n + 1›]
+    | succ {t₁ t₂: Term} (h₁: Eval₁ t₁ t₂): Eval₁ [Term| succ ‹t₁›] [Term| succ ‹t₂›]
+    | predZero: Eval₁ [Term| pred 0] [Term| 0]
+    | predSucc {v: Term} (h₁: Value v): Eval₁ [Term| pred succ ‹v›] [Term| ‹v›]
+    | pred {t₁ t₂: Term} (h₁: Eval₁ t₁ t₂): Eval₁ [Term| pred ‹t₁›] [Term| pred ‹t₂›]
+    | addL {t₁ t₂ t₃: Term} (h₁: Eval₁ t₁ t₂): Eval₁ [Term| ‹t₁› + ‹t₃›] [Term| ‹t₂› + ‹t₃›]
+    | addR {v₁ t₁ t₂: Term} (h₁: Value v₁) (h₂: Eval₁ t₁ t₂): Eval₁ [Term| ‹v₁› + ‹t₁›] [Term| ‹v₁› + ‹t₂›]
+    | add {n₁ n₂: Nat}: Eval₁ [Term| ‹nat:n₁› + ‹nat:n₂›] [Term| ‹nat:n₁ + n₂›]
+    | subL {t₁ t₂ t₃: Term} (h₁: Eval₁ t₁ t₂): Eval₁ [Term| ‹t₁› - ‹t₃›] [Term| ‹t₂› - ‹t₃›]
+    | subR {v₁ t₁ t₂: Term} (h₁: Value v₁) (h₂: Eval₁ t₁ t₂): Eval₁ [Term| ‹v₁› - ‹t₁›] [Term| ‹v₁› - ‹t₂›]
+    | sub {n₁ n₂: Nat}: Eval₁ [Term| ‹nat:n₁› - ‹nat:n₂›] [Term| ‹nat:n₁ - n₂›]
+    | mulL {t₁ t₂ t₃: Term} (h₁: Eval₁ t₁ t₂): Eval₁ [Term| ‹t₁› * ‹t₃›] [Term| ‹t₂› * ‹t₃›]
+    | mulR {v₁ t₁ t₂: Term} (h₁: Value v₁) (h₂: Eval₁ t₁ t₂): Eval₁ [Term| ‹v₁› * ‹t₁›] [Term| ‹v₁› * ‹t₂›]
+    | mul {n₁ n₂: Nat}: Eval₁ [Term| ‹nat:n₁› * ‹nat:n₂›] [Term| ‹nat:n₁ * n₂›]
+    | divL {t₁ t₂ t₃: Term} (h₁: Eval₁ t₁ t₂): Eval₁ [Term| ‹t₁› / ‹t₃›] [Term| ‹t₂› / ‹t₃›]
+    | divR {v₁ t₁ t₂: Term} (h₁: Value v₁) (h₂: Eval₁ t₁ t₂): Eval₁ [Term| ‹v₁› / ‹t₁›] [Term| ‹v₁› / ‹t₂›]
+    | div {n₁ n₂: Nat}: Eval₁ [Term| ‹nat:n₁› / ‹nat:n₂›] [Term| ‹nat:n₁ / n₂›]
+    | modL {t₁ t₂ t₃: Term} (h₁: Eval₁ t₁ t₂): Eval₁ [Term| ‹t₁› % ‹t₃›] [Term| ‹t₂› % ‹t₃›]
+    | modR {v₁ t₁ t₂: Term} (h₁: Value v₁) (h₂: Eval₁ t₁ t₂): Eval₁ [Term| ‹v₁› % ‹t₁›] [Term| ‹v₁› % ‹t₂›]
+    | mod {n₁ n₂: Nat}: Eval₁ [Term| ‹nat:n₁› % ‹nat:n₂›] [Term| ‹nat:n₁ % n₂›]
+    | expL {t₁ t₂ t₃: Term} (h₁: Eval₁ t₁ t₂): Eval₁ [Term| ‹t₁› ^ ‹t₃›] [Term| ‹t₂› ^ ‹t₃›]
+    | expR {v₁ t₁ t₂: Term} (h₁: Value v₁) (h₂: Eval₁ t₁ t₂): Eval₁ [Term| ‹v₁› ^ ‹t₁›] [Term| ‹v₁› ^ ‹t₂›]
+    | exp {n₁ n₂: Nat}: Eval₁ [Term| ‹nat:n₁› ^ ‹nat:n₂›] [Term| ‹nat:n₁ ^ n₂›]
+
+    | eqL {t₁ t₃ t₃: Term} (h₁: Eval₁ t₁ t₂): Eval₁ [Term| ‹t₁› = ‹t₃›] [Term| ‹t₂› = ‹t₃›]
+    | eqR {v₁ t₁ t₂: Term} (h₁: Value v₁) (h₂: Eval₁ t₁ t₂): Eval₁ [Term| ‹v₁› = ‹t₁›] [Term| ‹v₁› = ‹t₂›]
+    | eqTrue {v₁ v₂: Term} (h₁: Value v₁) (h₂: Value v₂) (h₃: Eq v₁ v₂): Eval₁ [Term| ‹v₁› = ‹v₂›] [Term| tru]
+    | eqFalse {v₁ v₂: Term} (h₁: Value v₁) (h₂: Value v₂) (h₃: ¬ Eq v₁ v₂): Eval₁ [Term| ‹v₁› = ‹v₂›] [Term| fls]
+    | neqL {t₁ t₃ t₃: Term} (h₁: Eval₁ t₁ t₂): Eval₁ [Term| ‹t₁› ≠ ‹t₃›] [Term| ‹t₂› ≠ ‹t₃›]
+    | neqR {v₁ t₁ t₂: Term} (h₁: Value v₁) (h₂: Eval₁ t₁ t₂): Eval₁ [Term| ‹v₁› ≠ ‹t₁›] [Term| ‹v₁› ≠ ‹t₂›]
+    | neqTrue {v₁ v₂: Term} (h₁: Value v₁) (h₂: Value v₂) (h₃: ¬ Eq v₁ v₂): Eval₁ [Term| ‹v₁› ≠ ‹v₂›] [Term| tru]
+    | neqFalse {v₁ v₂: Term} (h₁: Value v₁) (h₂: Value v₂) (h₃: Eq v₁ v₂): Eval₁ [Term| ‹v₁› ≠ ‹v₂›] [Term| fls]
+    | ltL {t₁ t₃ t₃: Term} (h₁: Eval₁ t₁ t₂): Eval₁ [Term| ‹t₁› < ‹t₃›] [Term| ‹t₂› < ‹t₃›]
+    | ltR {v₁ t₁ t₂: Term} (h₁: Value v₁) (h₂: Eval₁ t₁ t₂): Eval₁ [Term| ‹v₁› < ‹t₁›] [Term| ‹v₁› < ‹t₂›]
+    | ltTrue {n₁ n₂: Nat} (h₁: n₁ < n₂): Eval₁ [Term| ‹nat:n₁› < ‹nat:n₂›] [Term| tru]
+    | ltFalse {n₁ n₂: Nat} (h₁: n₁ ≥ n₂): Eval₁ [Term| ‹nat:n₁› < ‹nat:n₂›] [Term| fls]
+    | leL {t₁ t₃ t₃: Term} (h₁: Eval₁ t₁ t₂): Eval₁ [Term| ‹t₁› ≤ ‹t₃›] [Term| ‹t₂› ≤ ‹t₃›]
+    | leR {v₁ t₁ t₂: Term} (h₁: Value v₁) (h₂: Eval₁ t₁ t₂): Eval₁ [Term| ‹v₁› ≤ ‹t₁›] [Term| ‹v₁› ≤ ‹t₂›]
+    | leTrue {n₁ n₂: Nat} (h₁: n₁ ≤ n₂): Eval₁ [Term| ‹nat:n₁› ≤ ‹nat:n₂›] [Term| tru]
+    | leFalse {n₁ n₂: Nat} (h₁: n₁ > n₂): Eval₁ [Term| ‹nat:n₁› ≤ ‹nat:n₂›] [Term| fls]
+    | gtL {t₁ t₃ t₃: Term} (h₁: Eval₁ t₁ t₂): Eval₁ [Term| ‹t₁› > ‹t₃›] [Term| ‹t₂› > ‹t₃›]
+    | gtR {v₁ t₁ t₂: Term} (h₁: Value v₁) (h₂: Eval₁ t₁ t₂): Eval₁ [Term| ‹v₁› > ‹t₁›] [Term| ‹v₁› > ‹t₂›]
+    | gtTrue {n₁ n₂: Nat} (h₁: n₁ > n₂): Eval₁ [Term| ‹nat:n₁› > ‹nat:n₂›] [Term| tru]
+    | gtFalse {n₁ n₂: Nat} (h₁: n₁ ≤ n₂): Eval₁ [Term| ‹nat:n₁› > ‹nat:n₂›] [Term| fls]
+    | geL {t₁ t₃ t₃: Term} (h₁: Eval₁ t₁ t₂): Eval₁ [Term| ‹t₁› ≥ ‹t₃›] [Term| ‹t₂› ≥ ‹t₃›]
+    | geR {v₁ t₁ t₂: Term} (h₁: Value v₁) (h₂: Eval₁ t₁ t₂): Eval₁ [Term| ‹v₁› ≥ ‹t₁›] [Term| ‹v₁› ≥ ‹t₂›]
+    | geTrue {n₁ n₂: Nat} (h₁: n₁ ≥ n₂): Eval₁ [Term| ‹nat:n₁› ≥ ‹nat:n₂›] [Term| tru]
+    | geFalse {n₁ n₂: Nat} (h₁: n₁ < n₂): Eval₁ [Term| ‹nat:n₁› ≥ ‹nat:n₂›] [Term| fls]
+
+    | iteTrue {t f: Term}: Eval₁ [Term| ite tru then ‹t› else ‹f›] [Term| ‹t›]
+    | iteFalse {t f: Term}: Eval₁ [Term| ite fls then ‹t› else ‹f›] [Term| ‹f›]
+    | ite {c₁ c₂ t f: Term} (h₁: Eval₁ c₁ c₂): Eval₁ [Term| ite ‹c₁› then ‹t› else ‹f›] [Term| ite ‹c₂› then ‹t› else ‹f›]
+
+    | inl {t₁ t₂: Term} {ty: Ty} (h₁: Eval₁ t₁ t₂): Eval₁ [Term| inl (‹t₁› | ‹ty›)] [Term| inl (‹t₂› | ‹ty›)]
+    | inr {t₁ t₂: Term} {ty: Ty} (h₁: Eval₁ t₁ t₂): Eval₁ [Term| inr (‹ty› | ‹t₁›)] [Term| inr (‹ty› | ‹t₂›)]
+    | scaseInl {id₁ id₂: String} {t₁ t₂ t₃: Term} (h₁: Value t₁): Eval₁ [Term| case inl (‹t₁› | ‹ty›) of | inl ‹id₁› ⇒ ‹t₂› | inr ‹id₂› ⇒ ‹t₃›] ([id₁ ↦ t₁] [Term| ‹t₁›])
+    | scaseInr {id₁ id₂: String} {t₁ t₂ t₃: Term} (h₁: Value t₁): Eval₁ [Term| case inr (‹ty› | ‹t₁›) of | inl ‹id₁› ⇒ ‹t₂› | inr ‹id₂› ⇒ ‹t₃›] ([id₂ ↦ t₂] [Term| ‹t₂›])
+    | scase {id₁ id₂: String} {t₁ t₂ t₃ t₄: Term} (h₁: Eval₁ t₁ t₂): Eval₁ [Term| case ‹t₁› of | inl ‹id₁› ⇒ ‹t₃› | inr ‹id₂› ⇒ ‹t₄›] [Term| case ‹t₂› of | inl ‹id₁› ⇒ ‹t₃› | inr ‹id₂› ⇒ ‹t₄›]
+
+    | consL {t₁ t₂ t₃: Term} (h₁: Eval₁ t₁ t₂): Eval₁ [Term| ‹t₁› :: ‹t₃›] [Term| ‹t₂› :: ‹t₃›]
+    | consR {v₁ t₁ t₂: Term} (h₁: Value v₁) (h₂: Eval₁ t₁ t₂): Eval₁ [Term| ‹v₁› :: ‹t₁›] [Term| ‹v₁› :: ‹t₂›]
+    | lcaseNil {id₁ id₂: String} {t₁ t₂: Term}: Eval₁ [Term| case [] of | nil ⇒ ‹t₁› | ‹id₁› :: ‹id₂› ⇒ ‹t₂›] [Term| ‹t₁›]
+    | lcaseCons {id₁ id₂: String} {t₁ t₂ t₃ t₄: Term} (h₁: Value t₁) (h₂: Value t₂): Eval₁ [Term| case ‹t₁› :: ‹t₂› of | nil ⇒ ‹t₃› | ‹id₁› :: ‹id₂› ⇒ ‹t₄›] ([id₁ ↦ t₁] [id₂ ↦ t₂] [Term| ‹t₄›])
+    | lcase {id₁ id₂: String} {t₁ t₂ t₃ t₄: Term} (h₁: Eval₁ t₁ t₂): Eval₁ [Term| case ‹t₁› of | nil ⇒ ‹t₃› | ‹id₁› :: ‹id₂› ⇒ ‹t₄›] [Term| case ‹t₂› of | nil ⇒ ‹t₃› | ‹id₁› :: ‹id₂› ⇒ ‹t₄›]
+
+    | pairL {t₁ t₂ t₃: Term} (h₁: Eval₁ t₁ t₂): Eval₁ [Term| (‹t₁›, ‹t₃›)] [Term| (‹t₂›, ‹t₃›)]
+    | pairR {v₁ t₁ t₂: Term} (h₁: Value v₁) (h₂: Eval₁ t₁ t₂): Eval₁ [Term| (‹v₁›, ‹t₁›)] [Term| (‹v₁›, ‹t₂›)]
+    | fst {t₁ t₂: Term} (h₁: Value t₁) (h₂: Value t₂): Eval₁ [Term| fst (‹t₁›, ‹t₂›)] [Term| ‹t₁›]
+    | snd {t₁ t₂: Term} (h₁: Value t₁) (h₂: Value t₂): Eval₁ [Term| snd (‹t₁›, ‹t₂›)] [Term| ‹t₂›]
+    | pcaseVal {id₁ id₂: String} {t₁ t₂ t₃: Term} (h₁: Value t₁) (h₂: Value t₂): Eval₁ [Term| case (‹t₁›, ‹t₂›) of | (‹id₁›, ‹id₂›) ⇒ ‹t₃›] ([id₁ ↦ t₁] [id₂ ↦ t₂] [Term| ‹t₃›])
+    | pcase {id₁ id₂: String} {t₁ t₂ t₃: Term} (h₁: Eval₁ t₁ t₂): Eval₁ [Term| case ‹t₁› of | (‹id₁›, ‹id₂›) ⇒ ‹t₃›] [Term| case ‹t₂› of | (‹id₁›, ‹id₂›) ⇒ ‹t₃›]
+
+    | letL {id: String} {t₁ t₂ t₃: Term} (h₁: Eval₁ t₁ t₂): Eval₁ [Term| let ‹id› = ‹t₁› in ‹t₃›] [Term| let ‹id› = ‹t₂› in ‹t₃›]
+    | letR {id: String} {v₁ t₁ t₂: Term} (h₁: Value v₁) (h₂: Eval₁ ([id ↦ v₁] t₁) t₂): Eval₁ [Term| let ‹id› = ‹v₁› in ‹t₁›] [Term| let ‹id› = ‹v₁› in ‹t₂›]
+
+    | fix {t₁ t₂: Term} (h₁: Eval₁ t₁ t₂): Eval₁ [Term| fix ‹t₁›] [Term| fix ‹t₂›]
+    | fixAbs {id: String} {ty: Ty} {b: Term}: Eval₁ [Term| fix (λ ‹id›: ‹ty›. ‹b›)] ([id ↦ [Term| fix (λ ‹id›: ‹ty›. ‹b›)]] [Term| ‹b›])
+
+  scoped infix:50 "⟶" => Eval₁
+  scoped infix:50 "⇓"  => SmallStep.MultiStep Eval₁
+
+  /-
+  #### Typing
+  -/
+
+  open SoftwareFoundations.LogicalFoundations.Maps
+
+  def Context: Type := PartialMap Ty
+  def Context.empty: Context := PartialMap.empty
+
+  notation "●" => Context.empty
+  notation Γ ";" id ":" ty => PartialMap.update Γ id ty
+
+  inductive HasType: Context → Term → Ty → Prop where
+    | var {Γ: Context} {id: String} {ty: Ty} (h₁: Γ id = .some ty): HasType Γ [Term| ‹id:id›] [Ty| ‹ty›]
+    | abs {Γ: Context} {id: String} {ty₁ ty₂: Ty} {b: Term} (h₁: HasType (Γ; id: ty₁) b ty₂): HasType Γ [Term| λ ‹id›: ‹ty₁›. ‹b›] [Ty| ‹ty₁› → ‹ty₂›]
+    | app {Γ: Context} {t₁ t₂: Term} {ty₁ ty₂: Ty} (h₁: HasType Γ t₁ [Ty| ‹ty₁› → ‹ty₂›]) (h₂: HasType Γ t₂ [Ty| ‹ty₁›]): HasType Γ [Term| ‹t₁› ‹t₂›] [Ty| ‹ty₂›]
+
+    | true {Γ: Context}: HasType Γ [Term| tru] [Ty| 𝔹]
+    | false {Γ: Context}: HasType Γ [Term| fls] [Ty| 𝔹]
+    | and {Γ: Context} {t₁ t₂: Term} (h₁: HasType Γ t₁ [Ty| 𝔹]) (h₂: HasType Γ t₂ [Ty| 𝔹]): HasType Γ [Term| ‹t₁› ∧ ‹t₂›] [Ty| 𝔹]
+    | or {Γ: Context} {t₁ t₂: Term} (h₁: HasType Γ t₁ [Ty| 𝔹]) (h₂: HasType Γ t₂ [Ty| 𝔹]): HasType Γ [Term| ‹t₁› ∨ ‹t₂›] [Ty| 𝔹]
+    | not {Γ: Context} {t₁ t₂: Term} (h₁: HasType Γ t [Ty| 𝔹]): HasType Γ [Term| ¬ ‹t›] [Ty| 𝔹]
+    | bcase {Γ: Context} {c t f: Term} {ty: Ty} (h₁: HasType Γ c [Ty| 𝔹]) (h₂: HasType Γ t ty) (h₃: HasType Γ f ty): HasType Γ [Term| case ‹c› of | tru ⇒ ‹t› | fls ⇒ ‹f›] [Ty| ‹ty›]
+
+    | const {Γ: Context} {n: Nat}: HasType Γ [Term| ‹nat:n›] [Ty| ℕ]
+    | succ {Γ: Context} {t: Term} (h₁: HasType Γ t [Ty| ℕ]): HasType Γ [Term| succ ‹t›] [Ty| ℕ]
+    | pred {Γ: Context} {t: Term} (h₁: HasType Γ t [Ty| ℕ]): HasType Γ [Term| pred ‹t›] [Ty| ℕ]
+    | add {Γ: Context} {t₁ t₂: Term} (h₁: HasType Γ t₁ [Ty| ℕ]) (h₂: HasType Γ t₂ [Ty| ℕ]): HasType Γ [Term| ‹t₁› + ‹t₂›] [Ty| ℕ]
+    | sub {Γ: Context} {t₁ t₂: Term} (h₁: HasType Γ t₁ [Ty| ℕ]) (h₂: HasType Γ t₂ [Ty| ℕ]): HasType Γ [Term| ‹t₁› - ‹t₂›] [Ty| ℕ]
+    | mul {Γ: Context} {t₁ t₂: Term} (h₁: HasType Γ t₁ [Ty| ℕ]) (h₂: HasType Γ t₂ [Ty| ℕ]): HasType Γ [Term| ‹t₁› * ‹t₂›] [Ty| ℕ]
+    | div {Γ: Context} {t₁ t₂: Term} (h₁: HasType Γ t₁ [Ty| ℕ]) (h₂: HasType Γ t₂ [Ty| ℕ]): HasType Γ [Term| ‹t₁› / ‹t₂›] [Ty| ℕ]
+    | mod {Γ: Context} {t₁ t₂: Term} (h₁: HasType Γ t₁ [Ty| ℕ]) (h₂: HasType Γ t₂ [Ty| ℕ]): HasType Γ [Term| ‹t₁› % ‹t₂›] [Ty| ℕ]
+    | exp {Γ: Context} {t₁ t₂: Term} (h₁: HasType Γ t₁ [Ty| ℕ]) (h₂: HasType Γ t₂ [Ty| ℕ]): HasType Γ [Term| ‹t₁› ^ ‹t₂›] [Ty| ℕ]
+
+    | eq {Γ: Context} {t₁ t₂: Term} {ty: Ty} (h₁: HasType Γ t₁ ty) (h₂: HasType Γ t₂ ty): HasType Γ [Term| ‹t₁› = ‹t₂›] [Ty| ‹ty›]
+    | neq {Γ: Context} {t₁ t₂: Term} {ty: Ty} (h₁: HasType Γ t₁ ty) (h₂: HasType Γ t₂ ty): HasType Γ [Term| ‹t₁› ≠ ‹t₂›] [Ty| ‹ty›]
+    | lt {Γ: Context} {t₁ t₂: Term} (h₁: HasType Γ t₁ [Ty| ℕ]) (h₂: HasType Γ t₂ [Ty| ℕ]): HasType Γ [Term| ‹t₁› < ‹t₂›] [Ty| ℕ]
+    | le {Γ: Context} {t₁ t₂: Term} (h₁: HasType Γ t₁ [Ty| ℕ]) (h₂: HasType Γ t₂ [Ty| ℕ]): HasType Γ [Term| ‹t₁› ≤ ‹t₂›] [Ty| ℕ]
+    | gt {Γ: Context} {t₁ t₂: Term} (h₁: HasType Γ t₁ [Ty| ℕ]) (h₂: HasType Γ t₂ [Ty| ℕ]): HasType Γ [Term| ‹t₁› > ‹t₂›] [Ty| ℕ]
+    | ge {Γ: Context} {t₁ t₂: Term} (h₁: HasType Γ t₁ [Ty| ℕ]) (h₂: HasType Γ t₂ [Ty| ℕ]): HasType Γ [Term| ‹t₁› ≥ ‹t₂›] [Ty| ℕ]
+
+    | inl {Γ: Context} {t: Term} {ty₁ ty₂: Ty} (h₁: HasType Γ t ty₁): HasType Γ [Term| inl (‹t› | ‹ty₂›)] [Ty| ‹ty₁› + ‹ty₂›]
+    | inr {Γ: Context} {t: Term} {ty₁ ty₂: Ty} (h₁: HasType Γ t ty₂): HasType Γ [Term| inr (‹ty₁› | ‹t›)] [Ty| ‹ty₁› + ‹ty₂›]
+    | scase {Γ: Context} {c l r: Term} {id₁ id₂: String} {ty₁ ty₂ ty₃: Ty} (h₁: HasType Γ c [Ty| ‹ty₁› + ‹ty₂›]) (h₁: HasType (Γ; id₁: ty₁) l ty₃) (h₂: HasType (Γ; id₂: ty₂) r ty₃): HasType Γ [Term| case ‹c› of | inl ‹id₁› ⇒ ‹t₂› | inr ‹id₂› ⇒ ‹t₃›] [Ty| ‹ty₃›]
+
+    | nil {Γ: Context} {ty: Ty} (h₁: HasType Γ [Term| []] ty): HasType Γ [Term| []] [Ty| [‹ty›]]
+    | cons {Γ: Context} {hd tl: Term} {ty: Ty} (h₁: HasType Γ hd ty) (h₂: HasType Γ tl [Ty| [‹ty›]]): HasType Γ [Term| ‹hd› :: ‹tl›] [Ty| [‹ty›]]
+
+    | unit {Γ: Context}: HasType Γ [Term| ()] [Ty| ()]
+
+    | pair {Γ: Context} {t₁ t₂: Term} {ty₁ ty₂: Ty} (h₁: HasType Γ t₁ ty₁) (h₂: HasType Γ t₂ ty₂): HasType Γ [Term| (‹t₁›, ‹t₂›)] [Ty| ‹ty₁› × ‹ty₂›]
+    | fst {Γ: Context} {t: Term} {ty₁ ty₂: Ty} (h₁: HasType Γ t [Ty| ‹ty₁› × ‹ty₂›]): HasType Γ [Term| fst ‹t›] [Ty| ‹ty₁›]
+    | snd {Γ: Context} {t: Term} {ty₁ ty₂: Ty} (h₁: HasType Γ t [Ty| ‹ty₁› × ‹ty₂›]): HasType Γ [Term| snd ‹t›] [Ty| ‹ty₂›]
+    | pcase {Γ: Context} {c b: Term} {id₁ id₂: String} {ty₁ ty₂ ty₃: Ty} (h₁: HasType Γ c [Ty| ‹ty₁› × ‹ty₂›]) (h₂: HasType ((Γ; id₁: ty₁); id₂: ty₂) b ty₃): HasType Γ [Term| case ‹c› of | (‹id₁›, ‹id₂›) ⇒ ‹b›] [Ty| ‹t₃›]
+
+    | let {Γ: Context} {id: String} {t₁ t₂: Term} {ty₁ ty₂: Ty} (h₁: HasType Γ t₁ ty₁) (h₂: HasType (Γ; id: ty₁) t₂ ty₂): HasType Γ [Term| let ‹id› = ‹t₁› in ‹t₂›] [Ty| ‹ty₂›]
+
+    | fix {Γ: Context} {t: Term} {ty: Ty} (h₁: HasType Γ t [Ty| ‹ty› → ‹ty›]): HasType Γ [Term| fix ‹t›] [Ty| ‹ty›]
+
+  scoped notation ctx "⊢" t ":" ty => HasType ctx t ty
+
+  /-
+  ### Examples
+  -/
+
+  /-
+  #### Preliminaries
+  -/
+
+  /-
+  #### Numbers
+  -/
+
+  namespace NumTest
+    def testTerm := [Term|
+      ite (pred succ pred (2 * 0) = 0)
+      then 5
+      else 6
+    ]
+
+    namespace Term
+      example: ● ⊢ testTerm: [Ty| ℕ] := sorry
+      example: testTerm ⇓ [Term| 5] := sorry
+    end Term
+
+    namespace Tactic
+    end Tactic
+
+    namespace Blended
+    end Blended
+  end NumTest
+
+  /-
+  #### Products
+  -/
+
+  namespace ProdTest
+    def testTerm := [Term|
+      snd fst ((5, 6), 7)
+    ]
+
+    namespace Term
+      example: ● ⊢ testTerm: [Ty| ℕ] := sorry
+      example: testTerm ⇓ [Term| 6] := sorry
+    end Term
+
+    namespace Tactic
+    end Tactic
+
+    namespace Blended
+    end Blended
+  end ProdTest
+
+  /-
+  #### Let
+  -/
+
+  namespace LetTest
+    def testTerm₁ := [Term|
+      let x = pred 6 in
+      succ x
+    ]
+
+    def testTerm₂ := [Term|
+      let z = pred 6 in
+      succ z
+    ]
+
+    namespace Term
+      example: ● ⊢ testTerm₁: [Ty| ℕ] := sorry
+      example: testTerm₁ ⇓ [Term| 6] := sorry
+
+      example: ● ⊢ testTerm₂: [Ty| ℕ] := sorry
+      example: testTerm₂ ⇓ [Term| 6] := sorry
+    end Term
+
+    namespace Tactic
+    end Tactic
+
+    namespace Blended
+    end Blended
+  end LetTest
+
+  /-
+  #### Sums
+  -/
+
+  namespace SumTest
+    def testTerm₁ := [Term|
+      case inl (5 | ℕ) of
+        | inl x ⇒ x
+        | inr y ⇒ r
+    ]
+
+    def testTerm₂ := [Term|
+      let processSum = λ x: ℕ + ℕ.
+        case x of
+          | inl n ⇒ n
+          | inr n ⇒ ite n = 0 then 1 else 0
+      in
+      (processSum (inl (5 | ℕ)), processSum (inr (ℕ | 5)))
+    ]
+
+    namespace Term
+      example: ● ⊢ testTerm₁: [Ty| ℕ] := sorry
+      example: testTerm₁ ⇓ [Term| 5] := sorry
+
+      example: ● ⊢ testTerm₂: [Ty| ℕ × ℕ] := sorry
+      example: testTerm₂ ⇓ [Term| (5, 0)] := sorry
+    end Term
+
+    namespace Tactic
+    end Tactic
+
+    namespace Blended
+    end Blended
+  end SumTest
+
+  /-
+  #### Lists
+  -/
+
+  namespace ListTest
+    def testTerm := [Term|
+      let l = [5, 6] in
+      case l of
+        | nil ⇒ 0
+        | hd :: tl ⇒ hd * hd
+    ]
+
+    namespace Term
+      example: ● ⊢ testTerm: [Ty| ℕ] := sorry
+      example: testTerm ⇓ [Term| 25] := sorry
+    end Term
+
+    namespace Tactic
+    end Tactic
+
+    namespace Blended
+    end Blended
+  end ListTest
+
+  /-
+  #### Fix
+  -/
+
+  namespace FixTest
+    def fact := [Term|
+      fix (λ f: ℕ → ℕ. λ a: ℕ.
+        ite (a = 0)
+        then 1
+        else a * (f (pred a))
+      )
+    ]
+
+    def map := [Term|
+      λ g: ℕ → ℕ.
+        fix (λ f: [ℕ] → [ℕ]. λ l: [ℕ].
+          case l of
+            | nil ⇒ []
+            | hd :: tl ⇒ g hd :: f tl)
+    ]
+
+    def equal := [Term|
+      fix (λ eq: ℕ → ℕ → 𝔹. λ m: ℕ. λ n: ℕ.
+        ite m = 0
+        then ite n = 0
+             then tru
+             else fls
+        else ite n = 0
+             then fls
+             else eq (pred m) (pred n))
+    ]
+
+    def evenOdd := [Term|
+      let evenOdd = fix (λ evenOdd: ((ℕ → ℕ) × (ℕ → ℕ)).
+        ((λ n: ℕ. ite n = 0 then tru else (snd evenOdd) (pred n)),
+         (λ n: ℕ. ite n = 0 then fls else (fst evenOdd) (pred n)))
+      ) in
+      let even = fst evenOdd in
+      let odd = snd evenOdd in
+      (even 3, even 4)
+    ]
+
+    namespace Term
+      example: ● ⊢ fact: [Ty| ℕ → ℕ] := sorry
+      example: [Term| ‹fact› 4] ⇓ [Term| 24] := sorry
+
+      example: ● ⊢ map: [Ty| (ℕ → ℕ) → ([ℕ] → [ℕ])] := sorry
+      example: [Term| ‹map› (λ x: ℕ. succ x) [1, 2]] ⇓ [Term| 24] := sorry
+
+      example: ● ⊢ equal: [Ty| ℕ → ℕ → 𝔹] := sorry
+      example: [Term| ‹equal› 4 4] ⇓ [Term| tru] := sorry
+      example: [Term| ‹equal› 4 5] ⇓ [Term| fls] := sorry
+
+      example: ● ⊢ evenOdd: [Ty| 𝔹 × 𝔹] := sorry
+      example: evenOdd ⇓ [Term| (fls, tru)] := sorry
+    end Term
+
+    namespace Tactic
+    end Tactic
+
+    namespace Blended
+    end Blended
+  end FixTest
+
+  /-
+  ### Properties of Typing
+  -/
+
+  /-
+  #### Progress
+  -/
+
+  namespace Term
+    theorem HasType.progress {t₁: Term} {ty: Ty}: (● ⊢ t₁ : ty) → Value t ∨ ∃ t₂: Term, t₁ ⟶ t₂ := sorry
+  end Term
+
+  namespace Tactic
+  end Tactic
+
+  namespace Blended
+  end Blended
+
+  /-
+  #### Weakening
+  -/
+
+  namespace Term
+    theorem Context.weakening {Γ₁ Γ₂: Context} {t: Term} {ty: Ty}: Γ₁.includedIn Γ₂ → (Γ₁ ⊢ t : ty) → Γ₂ ⊢ t : ty := sorry
+    theorem Context.weakening.empty {Γ: Context} {t: Term} {ty: Ty}: (● ⊢ t : ty) → Γ ⊢ t : ty := sorry
+  end Term
+
+  namespace Tactic
+  end Tactic
+
+  namespace Blended
+  end Blended
+
+  /-
+  #### Substitution
+  -/
+
+  namespace Term
+    theorem Term.subst.preservation {Γ: Context} {id: String} {t₁ t₂: Term} {ty₁ ty₂: Ty}: (Γ.update id ty₁ ⊢ t₁ : ty₂) → (● ⊢ t₂ : ty₁) → Γ ⊢ (Term.subst id t₂ t₁) : ty₂ := sorry
+  end Term
+
+  namespace Tactic
+  end Tactic
+
+  namespace Blended
+  end Blended
+
+  /-
+  #### Preservation
+  -/
+
+  namespace Term
+    theorem HasType.preservation {t₁ t₂: Term} {ty: Ty}: (● ⊢ t₁ : ty) → (t₁ ⟶ t₂) → (● ⊢ t₂ : ty) := sorry
+  end Term
+
+  namespace Tactic
+  end Tactic
+
+  namespace Blended
+  end Blended
 end SoftwareFoundations.ProgrammingLanguageFoundations.MoreStlc
